\documentclass[../04-diophantine-equations.tex]{subfiles}

\begin{document}

\begin{example*}[\gls{USA 2015 MO}/P1]\label{example:USA-2015-MO-P1}[\textbf{\nameref{definition:15M}}]
	Giải trong tập số nguyên phương trình  
	\[
		x^2 + xy + y^2 \;=\; \Bigl(\frac{x+y}{3} + 1\Bigr)^3.
	\]
\end{example*}

\begin{story*}
    Start by letting \(x + y = 3t\). Substitute into the equation, simplify, and arrive at a form where \(4t + 1\) must be a perfect square. Let \(4t + 1 = (2n + 1)^2\), which leads to \(t = n^2 + n\). Solve for \(x\) and \(y\) in terms of \(n\), yielding the general solution for integer pairs \( (x, y) \).
\end{story*}

\bigbreak

\begin{soln}\footnotemark
	Đặt \(x+y=3t\). Khi đó:
	\[
		x^2 + xy + y^2 = (t+1)^3
		\quad\Longrightarrow\quad
		x^2 + x(3t - x) + (3t - x)^2 = (t+1)^3.
	\]
	Rút gọn và chuyển vế:
	\[
		(2x - 3t)^2 = (t - 2)^2 (4t + 1).
	\]
	Đặt \( 4t + 1 = (2n + 1)^2 \Rightarrow t = n^2 + n \). Thay vào:
	\[
		2x - 3(n^2 + n) = \pm\left( (n^2 + n - 2)(2n + 1) \right).
	\]
	Vế phải có thể rút gọn thành:
	\[
		2n^3 + 3n^2 - 3n - 2,
	\]
	và giải ra:
	\[
		x = n^3 + 3n^2 - 1 \quad \text{hoặc} \quad x = -n^3 + 3n + 1.
	\]
	Vì \( y = 3t - x = 3(n^2 + n) - x \), ta thu được hai cặp nghiệm đối xứng:
	\[
		(x, y) = \left(n^3 + 3n^2 - 1,\; -n^3 + 3n + 1\right)
		\quad \text{và} \quad
		(-n^3 + 3n + 1,\; n^3 + 3n^2 - 1),
	\]
	với mọi \( n \in \mathbb{Z} \).
\end{soln}

\footnotetext{\href{https://artofproblemsolving.com/wiki/index.php/2015_USAMO_Problems/Problem_1}{Lời giải chính thức.}}

\end{document}